src/FibEquiv.v
@@ -9,7 +9,9 @@ Require Import AST.
 Require Import Semantics.
 Require Import Utils.
 Require Import Builtins.
+Require Import Tactics.  
         
+Require Import ZArith.Znat.  
 
 Import HaskellListNotations.
 
@@ -20,18 +22,60 @@ Definition nz32 (n:Z) := @repr 32 nz n.
 Definition add32 (x y : Int) := @add 32 nz x y. 
 Definition sub32 (x y : Int) := @sub 32 nz x y. 
 
+
 (*
+Writing a Fib function over 32bit Ints doesn't appear to be fruitful since Coq doesn't believe that it terminates (since it doesn't for any negative argument). 
+
 Fixpoint fib (n : @Int 32) : (@Int 32) := 
   if (eq n (nz32 0)) then (nz32 1)
   else if (eq n (nz32 1)) then (nz32 1)
-  else add32 (fib (sub32 n (nz32 2))) (fib (sub32 n (nz32 1))). 
+  else add32 (fib (add32 n (nz32 (-1)))) (fib (add32 n (nz32(-2)))). 
 
-
-
-Theorem fib_equiv : forall n,
-   eval_expr fib_ge (Env n) (EApp (EVar fibnum) (EVar fibvar)) 
-   (bits (@repr width nz (fib n)). 
-
+Instead we will just define Fib over nats and then convert the result to a 32bit Int. Our equivalence theorem will have to have a restriction on the size of the input to take overflow into account
 *)
+
+Fixpoint fib (n : nat) : nat :=
+  match n with
+  | O  => S O 
+  | S n' => match n' with 
+         | O => S O
+         | S n'' => fib n' + fib n''
+  end
+end.
+
+(* Example of converting a fib result to 32bit Int *)
+Eval compute in (nz32 (Z.of_nat (fib 5))).   
+
+(* For the condition of the equiv theorem *)
+Definition Is_true (b:bool) :=
+  match b with
+    | true => True
+    | false => False
+  end.
+
+(* Just get the intval field in the Int record *)
+Definition Int32_to_Z (n : Int) : Z := @intval 32 n. 
+
+(* Lots of type conversion to say "Fib.cry n = fib n" *)
+Theorem fib_equiv : forall n, Is_true (ltu n (nz32 (@max_unsigned 32))) -> 
+   eval_expr fib_ge (Env (Int32_to_Z n)) (EApp (EVar fibnum) (EVar fibvar)) 
+   (bits (nz32 (Z.of_nat (fib (Z.to_nat (Int32_to_Z n)))))). 
+Proof. 
+  intros.  
+  e.
+  - global. e.
+  - local. 
+  - induction (Z.to_nat (Int32_to_Z n)). (* induction on n as a nat *)
+    + eapply eval_if_t. 
+    e. e. e. global. e. local. e. e. e. local. local.
+      * constructor; exact nz.
+      * e. 
+    + econstructor. e. e. e. global. e. local. e. e. e. local. local.
+      * destruct p. (* these aren't all true. Probably chose a constructor too early (eval_if_t) *)
+
+
+
+
+
 
 
